Observation Equation
V=Î¦(X_hat)-L
## Eq 
 
$$\begin{aligned} v_{1}=& \hat{x}-L_{1} \\ v_{2}=& \hat{x}-L_{2} \\ & \vdots \\ v_{n}=& \hat{x}-L_{n} \end{aligned}$$
$\sum_{i=1}^{n} p_{i} v_{i}^{2} \rightarrow \min$
 
 ## GM
 $\mathbf{v}_{n \times 1}=\mathbf{A}_{n \times u} \hat{\mathbf{x}}_{u \times 1}-\mathbf{L}_{n \times 1}$
 
## S
$\left[\begin{array}{l}\mathbf{l}_{N} \\ \mathbf{l}_{A}\end{array}\right]+\left[\begin{array}{l}\boldsymbol{v}_{N} \\ \boldsymbol{v}_{A}\end{array}\right]=\left[\begin{array}{cc}\boldsymbol{A}_{N} & \mathbf{A}_{A} \\ \mathbf{0} & \mathbf{I}_{A}\end{array}\right]\left[\begin{array}{c}\hat{\mathbf{x}}_{N} \\ \hat{\mathbf{x}}_{A}\end{array}\right]$

## GH
$y_i+v_{y_i}-a\left(x_i+v_{x_i}\right)-b=0$