## Lr
$\mathbf{v}=\mathbf{A} \hat{\mathbf{X}}-\mathbf{L}$
$\hat{\mathbf{L}}=\mathbf{L}+\mathbf{v}$


## GM

$\hat{\mathbf{X}}=\hat{\mathbf{X}}+\hat{\mathbf{x}}$
$\hat{\mathbf{v}}=\mathbf{A} \hat{\mathbf{x}}-\mathbf{l}$
$\hat{\mathbf{L}}=\mathbf{L_0}+\hat{\mathbf{v}}$

## L1
$P=1/v$

## S

$\hat{\mathbf{x}}=\left(\mathbf{A}^{\mathrm{T}} \mathbf{P} \mathbf{A}\right)^{-1} \mathbf{A}^{\mathrm{T}} \mathbf{P} \mathbf{l}=\mathbf{Q}_{\hat{x} \hat{x}} \mathbf{A}^{\mathrm{T}} \mathbf{P} \mathbf{l}$

$\mathbf{v}=\mathbf{A} \hat{\mathbf{x}}-\mathbf{l}$

## GH
$[\mathbf{k}]=\left[\mathbf{B} \mathbf{Q}_{l l} \mathbf{B}^{\mathrm{T}}\right]^{-1}[-\mathbf{w}]$
$\hat{\mathbf{X}}=\hat{\mathbf{X}}+\hat{\mathbf{x}}$
$\mathbf{v}=\mathbf{Q}_{l l} \mathbf{B}^{\mathrm{T}} k$
$\hat{\mathbf{L}}=\mathbf{L_0}+\hat{\mathbf{v}}$
## GH-con
$\hat{\mathbf{X}}=\hat{\mathbf{X}}+\hat{\mathbf{x}}$
$\mathbf{v}=\mathbf{Q}_{l l} \mathbf{B}^{\mathrm{T}} \mathbf{k}_1$
$\hat{\mathbf{L}}=\mathbf{L_0}+\hat{\mathbf{v}}$